proof/agp32UpdateScript.sml
@@ -6,7 +6,7 @@ val _ = new_theory "agp32Update";
 val _ = prefer_num ();
 val _ = guess_lengths ();
 
-(** a general lemma **)
+(** lemma about MAX_SET **)
 Theorem FINITE_max_ready_cycle:
   !t fext.
     FINITE {t0 | t0 < t /\ (fext t0).ready}
@@ -15,6 +15,33 @@ Proof
   `{t0 | t0 < t /\ (fext t0).ready} SUBSET (count t)` by rw [count_def,SUBSET_DEF] >>
   `FINITE (count t)` by fs [FINITE_COUNT] >>
   METIS_TAC [SUBSET_FINITE_I]
+QED
+
+Theorem same_t_and_m_under_MAX_SET_SUC:
+  !fext t m n.
+    MAX_SET {t0 | t0 < t /\ (fext t0).ready} = n ==>
+    (!p. p < m ==> ~(fext (p + (SUC n))).ready) ==>
+    (fext (m + SUC n)).ready ==>
+    ~(fext t).ready ==>
+    (fext (SUC t)).ready ==>
+    n <> 0 ==>
+    m + SUC n = SUC t
+Proof
+  rpt strip_tac >>
+  `FINITE {t0 | t0 < t /\ (fext t0).ready}` by fs [FINITE_max_ready_cycle] >>
+  Cases_on `{t0 | t0 < t /\ (fext t0).ready} = {}` >> fs [MAX_SET_DEF] >>
+  `n IN {t0 | t0 < t /\ (fext t0).ready}` by METIS_TAC [MAX_SET_DEF] >>
+  fs [MAX_SET_DEF] >>
+  Cases_on `m + SUC n = SUC t` >> fs [] >>
+  Cases_on `SUC t < m + SUC n` >-
+   (`SUC t -SUC n < m` by rw [] >>
+    `~(fext (SUC t -SUC n + SUC n)).ready` by fs [] >>
+    `SUC t -SUC n + SUC n = SUC t` by rw [] >> fs []) >>
+  `SUC t > m + SUC n` by fs [] >> fs [] >>
+  Cases_on `t = m + SUC n` >> fs [] >>
+  `t > m + SUC n` by fs [] >>
+  `(m + SUC n) IN {t0 | t0 < t /\ (fext t0).ready}` by fs [] >>
+  `(m + SUC n) <= n` by METIS_TAC [MAX_SET_DEF] >> fs []
 QED
 
 (* show the unchanged part of different circuit functions in the pipelined Silver *)
