proof/agp32_MEM_Data_CorrectScript.sml
@@ -1,0 +1,277 @@
+open hardwarePreamble translatorTheory translatorLib arithmeticTheory pred_setTheory wordsExtraTheory dep_rewrite blastLib bitstringSyntax fcpSyntax listSyntax wordsSyntax agp32StateTheory agp32EnvironmentTheory agp32ProcessorTheory ag32Theory ag32ExtraTheory ag32UtilitiesTheory agp32RelationTheory agp32UpdateTheory agp32InternalTheory agp32StepLib agp32_MEM_CorrectTheory;
+
+(* correctness of memory and data loading with respect to the ISA *)
+val _ = new_theory "agp32_MEM_Data_Correct";
+
+val _ = prefer_num ();
+val _ = guess_lengths ();
+
+
+(** memory **)
+Theorem agp32_Rel_ag32_fext_MEM_correct_MEM_not_NONE:
+  !fext fbits a t I.
+    is_mem fext_accessor_circuit (agp32 fext fbits) fext ==>
+    is_sch I (agp32 fext fbits) a ==>
+    Rel I (fext t) (agp32 fext fbits (t-1)) (agp32 fext fbits t) a t ==>
+    I (5,SUC t) <> NONE ==>
+    (fext (SUC t)).ready ==>
+    (fext (SUC t)).mem = (FUNPOW Next (THE (I (5,SUC t))) a).MEM
+Proof
+  rw [] >> cheat
+QED
+
+(** data_rdata **)
+(** LoadMem **)
+(** WB enabled **)
+Theorem agp32_Rel_ag32_read_mem_data_rdata_correct_WB_enable:
+  !fext fbits a t I.
+    is_mem fext_accessor_circuit (agp32 fext fbits) fext ==>
+    is_sch I (agp32 fext fbits) a ==>
+    Rel I (fext t) (agp32 fext fbits (t-1)) (agp32 fext fbits t) a t ==>
+    I (5,SUC t) <> NONE ==>
+    (fext (SUC t)).ready ==>
+    (agp32 fext fbits (SUC t)).WB.WB_opc = 4w ==>
+    enable_stg 5 (agp32 fext fbits t) ==>
+    (fext (SUC t)).data_rdata = mem_data_rdata (FUNPOW Next (THE (I (5,SUC t)) - 1) a)
+Proof
+  rw [] >> `I' (5,SUC t) = I' (4,t)` by fs [is_sch_def,is_sch_writeback_def] >>
+  `align_addr (agp32 fext fbits (SUC t)).data_addr =
+  mem_data_addr (FUNPOW Next (THE (I' (5,SUC t)) - 1) a)`
+    by METIS_TAC [agp32_Rel_ag32_data_addr_correct_read_mem] >>
+  `(agp32 fext fbits t).MEM.MEM_opc = 4w` by METIS_TAC [agp32_WB_opc_MEM_opc_when_WB_enabled] >>
+  `(agp32 fext fbits t).MEM.MEM_read_mem` by METIS_TAC [agp32_MEM_read_mem_MEM_opc_4w_5w] >>
+  `opc (FUNPOW Next (THE (I' (4,t)) - 1) a) = 4w` by fs [Rel_def,MEM_Rel_def] >>
+  fs [mem_data_rdata_def] >>
+  `(fext t).ready` by (fs [enable_stg_def] >> METIS_TAC [agp32_WB_state_flag_and_fext_ready]) >>
+  last_assum (assume_tac o is_mem_def_mem_no_errors) >>
+  `(agp32 fext fbits (SUC t)).command = 2w`
+    by METIS_TAC [agp32_Rel_ag32_command_correct_read_mem_WB_enable] >>
+  last_assum (mp_tac o is_mem_data_read `SUC t`) >> rw [] >>
+  Cases_on `m` >> fs [] >-
+   (fs [Rel_def] >>
+    Cases_on `I' (5,t) = NONE` >> fs [] >>
+    `THE (I' (4,t)) = THE (I' (5,t)) + 1`
+      by METIS_TAC [MEM_instr_index_with_WB_instr_plus_1] >> fs []) >>
+  `~(fext (0 + SUC t)).ready` by fs [] >> fs []
+QED
+
+(** WB is disabled and fext is not ready at the previous cycle **)
+(** lemma **)
+Theorem WB_opc_unchanged_after_disabled_cycles[local]:
+  !fext fbits m n.
+    (!p. p < m ==> ~(fext (p + n)).ready) ==>
+    (agp32 fext fbits (m + n)).WB.WB_opc = (agp32 fext fbits n).WB.WB_opc
+Proof
+  rw [] >> Induct_on `m` >> rw [] >>
+  `!p. p < m ==> ~(fext (n + p)).ready` by fs [] >> fs [] >>
+  `m < SUC m` by rw [] >>
+  `~(fext (n + m)).ready` by fs [] >>
+  `~(agp32 fext fbits (n + m)).WB.WB_state_flag`
+    by METIS_TAC [agp32_WB_state_flag_and_fext_ready] >>
+  `(agp32 fext fbits (SUC (n + m))).WB.WB_opc = (agp32 fext fbits (n + m)).WB.WB_opc`
+    by fs [agp32_WB_opc_unchanged_when_WB_disabled,enable_stg_def] >>
+  `n + SUC m = SUC (n + m)` by rw [] >> rw [] >> fs []
+QED
+
+Theorem data_addr_unchanged_after_disabled_cycles[local]:
+  !fext fbits m n.
+    (!p. p < m ==> ~(fext (p + n)).ready) ==>
+    (agp32 fext fbits (m + n)).data_addr = (agp32 fext fbits n).data_addr
+Proof
+  rw [] >> Induct_on `m` >> rw [] >>
+  `!p. p < m ==> ~(fext (n + p)).ready` by fs [] >> fs [] >>
+  `m < SUC m` by rw [] >>
+  `~(fext (n + m)).ready` by fs [] >>
+  `~(agp32 fext fbits (n + m)).WB.WB_state_flag`
+    by METIS_TAC [agp32_WB_state_flag_and_fext_ready] >>
+  `(agp32 fext fbits (SUC (n + m))).data_addr = (agp32 fext fbits (n + m)).data_addr`
+    by fs [agp32_data_addr_wstrb_wdata_unchanged_when_WB_disabled,enable_stg_def] >>
+  `n + SUC m = SUC (n + m)` by rw [] >> rw [] >> fs []
+QED
+
+Theorem WB_opc_unchanged_after_disabled_cycles_0[local]:
+  !fext fbits m.
+    (!p. p < m ==> ~(fext p).ready) ==>
+    (agp32 fext fbits m).WB.WB_opc = (agp32 fext fbits 0).WB.WB_opc
+Proof
+  rw [] >> `!p. p < m ==> ~(fext (p + 0)).ready` by fs [] >>
+  `(agp32 fext fbits (m + 0)).WB.WB_opc = (agp32 fext fbits 0).WB.WB_opc`
+    by fs [WB_opc_unchanged_after_disabled_cycles] >> fs []
+QED
+
+Theorem EMPTY_no_fext_ready_cycle[local]:
+  !t fext.
+    {t0 | t0 < t /\ (fext t0).ready} = {} ==>
+    (!t0. t0 < t ==> ~(fext t0).ready)
+Proof
+  rw [] >> Cases_on `(fext t0).ready` >> rw [] >>
+  `t0 IN {t0 | t0 < t /\ (fext t0).ready}` by fs [] >>
+  METIS_TAC [MEMBER_NOT_EMPTY]
+QED
+
+Theorem MAX_SET_0_no_fext_ready_cycle[local]:
+  !t fext.
+    {t0 | t0 < t /\ (fext t0).ready} <> {} ==>
+    MAX_SET {t0 | t0 < t /\ (fext t0).ready} = 0 ==>
+    (!t0. t0 < t - 1 ==> ~(fext (t0 + 1)).ready)
+Proof
+  rw [] >>
+  `FINITE {t0 | t0 < t /\ (fext t0).ready}` by rw [FINITE_max_ready_cycle] >>
+  Cases_on `(fext (t0 + 1)).ready` >> rw [] >>
+  `t0 + 1  < t` by fs [] >>
+  `t0 + 1 IN {t0 | t0 < t /\ (fext t0).ready}` by fs [] >>
+  `t0 + 1 <= 0` by METIS_TAC [MAX_SET_DEF] >> rw []
+QED
+
+Theorem agp32_Rel_ag32_read_mem_data_rdata_correct_WB_disable_fext_not_ready:
+  !fext fbits a t I.
+    is_mem fext_accessor_circuit (agp32 fext fbits) fext ==>
+    is_sch I (agp32 fext fbits) a ==>
+    Rel I (fext t) (agp32 fext fbits (t-1)) (agp32 fext fbits t) a t ==>
+    I (5,SUC t) <> NONE ==>
+    (fext (SUC t)).ready ==>
+    ~(fext t).ready ==>
+    (agp32 fext fbits (SUC t)).WB.WB_opc = 4w ==>
+    ~enable_stg 5 (agp32 fext fbits t) ==>
+    (fext (SUC t)).data_rdata = mem_data_rdata (FUNPOW Next (THE (I (5,SUC t)) - 1) a)
+Proof
+  rw [] >> Cases_on `MAX_SET {t0 | t0 < t /\ (fext t0).ready}` >-
+   (Cases_on `{t0 | t0 < t /\ (fext t0).ready} = {}` >-
+     (`!t0. t0 < t ==> ~(fext t0).ready` by METIS_TAC [EMPTY_no_fext_ready_cycle] >>
+      `(agp32 fext fbits t).WB.WB_opc = (agp32 fext fbits 0).WB.WB_opc`
+        by fs [WB_opc_unchanged_after_disabled_cycles_0] >>
+      fs [agp32_WB_opc_unchanged_when_WB_disabled,agp32_init_WB_opc]) >>
+    `!t0. t0 < t - 1 ==> ~(fext (t0 + 1)).ready`
+      by METIS_TAC [MAX_SET_0_no_fext_ready_cycle] >>
+    `(agp32 fext fbits (t - 1 + 1)).WB.WB_opc = (agp32 fext fbits 1).WB.WB_opc`
+      by fs [WB_opc_unchanged_after_disabled_cycles] >>
+    `t - 1 + 1 = t` by (Cases_on `t` >> fs []) >> fs [] >>
+    `(agp32 fext fbits t).WB.WB_opc = 4w` by fs [agp32_WB_opc_unchanged_when_WB_disabled] >>
+    `~enable_stg 5 (agp32 fext fbits 0)` by fs [agp32_init_ctrl_flags,enable_stg_def] >>
+    `(agp32 fext fbits (SUC 0)).WB.WB_opc = 16w`
+      by fs [agp32_WB_opc_unchanged_when_WB_disabled,agp32_init_WB_opc] >>
+    fs [SUC_ONE_ADD]) >>
+  Q.ABBREV_TAC `i = SUC n` >> `i <> 0` by fs [Abbr `i`] >>
+  `FINITE {t0 | t0 < t /\ (fext t0).ready}` by fs [FINITE_max_ready_cycle] >>
+  Cases_on `{t0 | t0 < t /\ (fext t0).ready} = {}` >> fs [MAX_SET_DEF] >>
+  `i IN {t0 | t0 < t /\ (fext t0).ready}` by METIS_TAC [MAX_SET_DEF] >> fs [MAX_SET_DEF] >>
+  last_assum (assume_tac o is_mem_def_mem_no_errors) >>
+  Cases_on_word_value `(agp32 fext fbits (SUC i)).command` >>
+  fs [agp32_command_impossible_values] >-
+   (last_assum (mp_tac o is_mem_data_flush `SUC i`) >> simp [] >> strip_tac >>
+    `m + SUC i = SUC t` by METIS_TAC [same_t_and_m_under_MAX_SET_SUC] >> fs [] >>
+    cheat) >-
+   (last_assum (mp_tac o is_mem_data_write `SUC i`) >> simp [] >> strip_tac >>
+    `m + SUC i = SUC t` by METIS_TAC [same_t_and_m_under_MAX_SET_SUC] >> fs [] >>
+    cheat) >-
+   (last_assum (mp_tac o is_mem_data_read `SUC i`) >> simp [] >> strip_tac >>
+    `m + SUC i = SUC t` by METIS_TAC [same_t_and_m_under_MAX_SET_SUC] >> fs [] >>
+    `(fext (SUC t)).mem = (FUNPOW Next (THE (I' (5,SUC t))) a).MEM`
+       by METIS_TAC [agp32_Rel_ag32_fext_MEM_correct_MEM_not_NONE] >>
+    `I' (5,SUC t) = I' (5,t)` by fs [is_sch_def,is_sch_disable_def] >> fs [] >>
+    `(agp32 fext fbits (SUC t)).WB.WB_opc = (agp32 fext fbits t).WB.WB_opc`
+      by fs [agp32_WB_opc_unchanged_when_WB_disabled] >>
+    `opc (FUNPOW Next (THE (I' (5,t)) - 1) a) = 4w` by fs [Rel_def,WB_Rel_def] >>
+    simp [mem_data_rdata_def] >>
+    `(agp32 fext fbits (SUC i)).data_addr = (agp32 fext fbits (m + SUC i)).data_addr`
+      by METIS_TAC [data_addr_unchanged_after_disabled_cycles] >>
+    `align_addr (agp32 fext fbits (SUC t)).data_addr =
+    mem_data_addr (FUNPOW Next (THE (I' (5,SUC t)) - 1) a)`
+      by METIS_TAC [agp32_Rel_ag32_data_addr_correct_read_mem] >>
+    `align_addr (agp32 fext fbits (SUC i)).data_addr =
+    mem_data_addr (FUNPOW Next (THE (I' (5,t)) - 1) a)` by fs [Rel_def] >> fs [] >>
+    `(fext (SUC i)).mem = (fext i).mem`
+      by (Cases_on `m` >> fs [] >> `0 < SUC n` by rw [] >>
+          `(fext (0 + SUC i)).mem = (fext i).mem` by fs [] >> fs []) >>
+    `(fext (SUC i)).mem = (fext (SUC t)).mem` by fs [] >> fs [] >>
+    `~is_wrMEM_isa (FUNPOW Next (THE (I' (5,t)) - 1) a)` by fs [is_wrMEM_isa_def] >>
+    METIS_TAC [word_at_addr_not_changed_after_normal_instrs]) >-
+   (last_assum (mp_tac o is_mem_inst_read `SUC i`) >> simp [] >> strip_tac >>
+    `m + SUC i = SUC t` by METIS_TAC [same_t_and_m_under_MAX_SET_SUC] >> fs [] >>
+    cheat) >>
+  last_assum (mp_tac o is_mem_do_nothing `SUC i`) >> simp [] >> strip_tac >>
+  Cases_on `SUC i = t` >> fs [] >>
+  Cases_on `SUC i > t` >> fs [] >>
+  `SUC i < t` by fs [] >>
+  `(SUC i) IN {t0 | t0 < t /\ (fext t0).ready}` by fs [] >>
+  `(SUC i) <= i` by METIS_TAC [MAX_SET_DEF] >> fs []
+QED
+
+(** WB disabled **) 
+Theorem agp32_Rel_ag32_read_mem_data_rdata_correct_WB_disable:
+  !fext fbits a t I.
+    is_mem fext_accessor_circuit (agp32 fext fbits) fext ==>
+    is_sch I (agp32 fext fbits) a ==>
+    Rel I (fext t) (agp32 fext fbits (t-1)) (agp32 fext fbits t) a t ==>
+    I (5,SUC t) <> NONE ==>
+    (fext (SUC t)).ready ==>
+    (agp32 fext fbits (SUC t)).WB.WB_opc = 4w ==>
+    ~enable_stg 5 (agp32 fext fbits t) ==>
+    (fext (SUC t)).data_rdata = mem_data_rdata (FUNPOW Next (THE (I (5,SUC t)) - 1) a)
+Proof
+  rw [] >> Cases_on `(fext t).ready` >-
+   (`I' (5,SUC t) = I' (5,t)` by fs [is_sch_def,is_sch_disable_def] >>
+    `(agp32 fext fbits (SUC t)).WB.WB_opc = (agp32 fext fbits t).WB.WB_opc`
+      by fs [agp32_WB_opc_unchanged_when_WB_disabled] >>
+    last_assum (assume_tac o is_mem_def_mem_no_errors) >>
+    Cases_on_word_value `(agp32 fext fbits (SUC t)).command` >>
+    fs [agp32_command_impossible_values] >-
+     (last_assum (mp_tac o is_mem_data_flush `SUC t`) >> rw [] >>
+      Cases_on `m` >> fs [] >-
+       fs [Rel_def,MEM_data_rel_def] >>
+      `~(fext (0 + SUC t)).ready` by fs [] >> fs []) >-
+     (last_assum (mp_tac o is_mem_data_write `SUC t`) >> rw [] >>
+      Cases_on `m` >> fs [] >-
+       fs [Rel_def,MEM_data_rel_def] >>
+      `~(fext (0 + SUC t)).ready` by fs [] >> fs []) >-
+     (last_assum (mp_tac o is_mem_data_read `SUC t`) >> rw [] >>
+      Cases_on `m` >> fs [] >-
+       (`opc (FUNPOW Next (THE (I' (5,t)) - 1) a) = 4w` by fs [Rel_def,WB_Rel_def] >>
+        rw [mem_data_rdata_def] >>
+        `align_addr (agp32 fext fbits (SUC t)).data_addr =
+        mem_data_addr (FUNPOW Next (THE (I' (5,SUC t)) - 1) a)`
+          by METIS_TAC [agp32_Rel_ag32_data_addr_correct_read_mem] >>
+        fs [Rel_def] >>
+        `~is_wrMEM_isa (FUNPOW Next (THE (I' (5,t)) - 1) a)` by fs [is_wrMEM_isa_def] >>
+        METIS_TAC [word_at_addr_not_changed_after_normal_instrs]) >>
+      `~(fext (0 + SUC t)).ready` by fs [] >> fs []) >-
+     (last_assum (mp_tac o is_mem_inst_read `SUC t`) >> rw [] >>
+      Cases_on `m` >> fs [] >-
+       fs [Rel_def,MEM_data_rel_def] >>
+      `~(fext (0 + SUC t)).ready` by fs [] >> fs []) >>
+    last_assum (mp_tac o is_mem_do_nothing `SUC t`) >> rw [] >>
+    fs [Rel_def,MEM_data_rel_def]) >>
+  METIS_TAC [agp32_Rel_ag32_read_mem_data_rdata_correct_WB_disable_fext_not_ready]
+QED
+
+Theorem agp32_Rel_ag32_read_mem_data_rdata_correct:
+  !fext fbits a t I.
+    is_mem fext_accessor_circuit (agp32 fext fbits) fext ==>
+    is_sch I (agp32 fext fbits) a ==>
+    Rel I (fext t) (agp32 fext fbits (t-1)) (agp32 fext fbits t) a t ==>
+    I (5,SUC t) <> NONE ==>
+    (fext (SUC t)).ready ==>
+    (agp32 fext fbits (SUC t)).WB.WB_opc = 4w ==>
+    (fext (SUC t)).data_rdata = mem_data_rdata (FUNPOW Next (THE (I (5,SUC t)) - 1) a)
+Proof
+  rw [] >> Cases_on `enable_stg 5 (agp32 fext fbits t)` >>
+  METIS_TAC [agp32_Rel_ag32_read_mem_data_rdata_correct_WB_enable,
+             agp32_Rel_ag32_read_mem_data_rdata_correct_WB_disable]
+QED
+
+
+(* MEM_data_rel *)
+Theorem agp32_Rel_ag32_MEM_data_rel_correct:
+  !fext fbits a t I.
+    is_mem fext_accessor_circuit (agp32 fext fbits) fext ==>
+    is_sch I (agp32 fext fbits) a ==>
+    Rel I (fext t) (agp32 fext fbits (t-1)) (agp32 fext fbits t) a t ==>
+    I (5,SUC t) <> NONE ==>
+    MEM_data_rel (fext (SUC t)) (agp32 fext fbits (SUC t)) a (THE (I (5,SUC t)))
+Proof
+  rw [MEM_data_rel_def] >-
+   METIS_TAC [agp32_Rel_ag32_read_mem_data_rdata_correct] >>
+  cheat
+QED
+
+val _ = export_theory ();
